@prefix : <http://www.semanticweb.org/user/ontologies/2022/10/untitled-ontology-328#> .
@prefix owl: <http://www.w3.org/2002/07/owl#> .
@prefix rdf: <http://www.w3.org/1999/02/22-rdf-syntax-ns#> .
@prefix xml: <http://www.w3.org/XML/1998/namespace> .
@prefix xsd: <http://www.w3.org/2001/XMLSchema#> .
@prefix rdfs: <http://www.w3.org/2000/01/rdf-schema#> .
@base <http://www.semanticweb.org/user/ontologies/2022/10/untitled-ontology-328> .

<http://www.semanticweb.org/user/ontologies/2022/10/untitled-ontology-328> rdf:type owl:Ontology .

#################################################################
#    Object Properties
#################################################################

###  http://www.semanticweb.org/user/ontologies/2022/10/untitled-ontology-328#hasColour
:hasColour rdf:type owl:ObjectProperty ;
           rdfs:subPropertyOf :hasSymptoms ;
           rdfs:domain :CancerType ;
           rdfs:range :Symptom ;
           rdfs:comment "A property that indicates the colour of the instance (i.e., skin cancer or potenital skin cancer)" ;
           rdfs:label "has colour" .


###  http://www.semanticweb.org/user/ontologies/2022/10/untitled-ontology-328#hasDanger
:hasDanger rdf:type owl:ObjectProperty ;
           rdfs:domain :CancerType ;
           rdfs:range :Danger ;
           rdfs:comment "A property that indicates the dangers which increase the risk to suffer skin cancer" ;
           rdfs:label "has danger" .


###  http://www.semanticweb.org/user/ontologies/2022/10/untitled-ontology-328#hasShape
:hasShape rdf:type owl:ObjectProperty ;
          rdfs:subPropertyOf :hasSymptoms ;
          rdfs:domain :CancerType ;
          rdfs:range :Symptom ;
          rdfs:comment "A property that indicates the shape of the instance (i.e., skin cancer or potenital skin cancer)" ;
          rdfs:label "has shape" .


###  http://www.semanticweb.org/user/ontologies/2022/10/untitled-ontology-328#hasSize
:hasSize rdf:type owl:ObjectProperty ;
         rdfs:subPropertyOf :hasSymptoms ;
         rdfs:domain :CancerType ;
         rdfs:range :Symptom ;
         rdfs:comment "A property that indicates the size of the instance (i.e., skin cancer or potenital skin cancer)" ;
         rdfs:label "hasSize" .


###  http://www.semanticweb.org/user/ontologies/2022/10/untitled-ontology-328#hasState
:hasState rdf:type owl:ObjectProperty ;
          rdfs:subPropertyOf :hasSymptoms ;
          rdfs:domain :CancerType ;
          rdfs:range :Symptom ;
          rdfs:comment "A property that indicates the state of the instance (i.e., skin cancer or potenital skin cancer)" ;
          rdfs:label "has state" .


###  http://www.semanticweb.org/user/ontologies/2022/10/untitled-ontology-328#hasSymptoms
:hasSymptoms rdf:type owl:ObjectProperty ;
             rdfs:domain :CancerType ;
             rdfs:range :Symptom ;
             rdfs:comment "A property that indicatesthe sympotms the instance (i.e., skin cancer or potenital skin cancer) has" ;
             rdfs:label "has symptoms" .


###  http://www.semanticweb.org/user/ontologies/2022/10/untitled-ontology-328#inBodyCharacteristic
:inBodyCharacteristic rdf:type owl:ObjectProperty ;
                      rdfs:subPropertyOf :hasDanger ;
                      rdfs:domain :CancerType ;
                      rdfs:range :BodyCharacteristic ;
                      rdfs:comment "A property that indicates the body characteristics which increase the risk to suffer skin cancer" ;
                      rdfs:label "in body characteristic" .


###  http://www.semanticweb.org/user/ontologies/2022/10/untitled-ontology-328#inExposure
:inExposure rdf:type owl:ObjectProperty ;
            rdfs:subPropertyOf :hasDanger ;
            rdfs:domain :CancerType ;
            rdfs:range :Exposure ;
            rdfs:comment "A property that indicates the exposures which increase the risk to suffer skin cancer" ;
            rdfs:label "in exposure" .


###  http://www.semanticweb.org/user/ontologies/2022/10/untitled-ontology-328#inFamilyHistory
:inFamilyHistory rdf:type owl:ObjectProperty ;
                 rdfs:subPropertyOf :hasDanger ;
                 rdfs:domain :CancerType ;
                 rdfs:range :FamilyHistory ;
                 rdfs:comment "A property that indicates the family history which increase the risk to suffer skin cancer" ;
                 rdfs:label "in family history" .


###  http://www.semanticweb.org/user/ontologies/2022/10/untitled-ontology-328#inImmuneSystem
:inImmuneSystem rdf:type owl:ObjectProperty ;
                rdfs:subPropertyOf :hasDanger ;
                rdfs:domain :CancerType ;
                rdfs:range :ImmuneSystem ;
                rdfs:comment "A property that indicates the immune system states which increase the risk to suffer skin cancer" ;
                rdfs:label "in immune system" .


###  http://www.semanticweb.org/user/ontologies/2022/10/untitled-ontology-328#inSkinType
:inSkinType rdf:type owl:ObjectProperty ;
            rdfs:subPropertyOf :hasDanger ;
            rdfs:domain :CancerType ;
            rdfs:range :SkinType ;
            rdfs:comment "A property that indicates the skin types which increase the risk to suffer skin cancer" ;
            rdfs:label "in skin type" .


###  http://www.semanticweb.org/user/ontologies/2022/10/untitled-ontology-328#isLocated
:isLocated rdf:type owl:ObjectProperty ;
           rdfs:domain :CancerType ;
           rdfs:range :BodyPart ;
           rdfs:comment "A property that indicates in which body part the instance (i.e., skin cancer or potenital skin cancer) is located" ;
           rdfs:label "is located" .


#################################################################
#    Data properties
#################################################################

###  http://www.semanticweb.org/user/ontologies/2022/10/untitled-ontology-328#colour
:colour rdf:type owl:DatatypeProperty ;
        rdfs:domain :Colour ,
                    :SkinType ;
        rdfs:range xsd:string ;
        rdfs:comment "A property that indiciates the colour of an instance. Instance is an entity that could be skin cancer or not" ;
        rdfs:label "colour" .


###  http://www.semanticweb.org/user/ontologies/2022/10/untitled-ontology-328#exposureTo
:exposureTo rdf:type owl:DatatypeProperty ;
            rdfs:domain :Exposure ;
            rdfs:range xsd:string ;
            rdfs:comment "A property that indicates to what  an individual has been exposed" ;
            rdfs:label "exposure to" .


###  http://www.semanticweb.org/user/ontologies/2022/10/untitled-ontology-328#geneChange
:geneChange rdf:type owl:DatatypeProperty ;
            rdfs:domain :FamilyHistory ;
            rdfs:range xsd:string ;
            rdfs:comment "A property that indicates if an individual had some gene changes in the past" ;
            rdfs:label "gene change" .


###  http://www.semanticweb.org/user/ontologies/2022/10/untitled-ontology-328#getsBurn
:getsBurn rdf:type owl:DatatypeProperty ;
          rdfs:domain :SkinType ;
          rdfs:range xsd:string ;
          rdfs:label "A property that indiciates if a skin type gets often burns or not" ,
                     "gets burn" .


###  http://www.semanticweb.org/user/ontologies/2022/10/untitled-ontology-328#hadBasalCellCarcinoma
:hadBasalCellCarcinoma rdf:type owl:DatatypeProperty ;
                       rdfs:domain :FamilyHistory ;
                       rdfs:range xsd:boolean ;
                       rdfs:comment "A property that indicates if an individual had a basal cell carcinoma in the past" ;
                       rdfs:label "has basal cell carcinoma" .


###  http://www.semanticweb.org/user/ontologies/2022/10/untitled-ontology-328#hadSquamousCellCarcinoma
:hadSquamousCellCarcinoma rdf:type owl:DatatypeProperty ;
                          rdfs:domain :FamilyHistory ;
                          rdfs:range xsd:boolean ;
                          rdfs:comment "A property that indicates if an individual had a squamous cell carcinoma in the past" ;
                          rdfs:label "squamous cell carcinoma" .


###  http://www.semanticweb.org/user/ontologies/2022/10/untitled-ontology-328#hadSunburnBlister
:hadSunburnBlister rdf:type owl:DatatypeProperty ;
                   rdfs:domain :FamilyHistory ;
                   rdfs:range xsd:boolean ;
                   rdfs:comment "A property that indicates if an individual had sunburn blisters in the past" ;
                   rdfs:label "had sunburn blister" .


###  http://www.semanticweb.org/user/ontologies/2022/10/untitled-ontology-328#hadSyndrome
:hadSyndrome rdf:type owl:DatatypeProperty ;
             rdfs:domain :FamilyHistory ;
             rdfs:range xsd:string ;
             rdfs:comment "A property that indicates if the individual has a specific syndrome or not" ;
             rdfs:label "xsd:string" .


###  http://www.semanticweb.org/user/ontologies/2022/10/untitled-ontology-328#hadUnusualMole
:hadUnusualMole rdf:type owl:DatatypeProperty ;
                rdfs:domain :FamilyHistory ;
                rdfs:range xsd:boolean ;
                rdfs:comment "A property that indicates if an individual had an unusual mole" ;
                rdfs:label "had unusual mole" .


###  http://www.semanticweb.org/user/ontologies/2022/10/untitled-ontology-328#hasAge
:hasAge rdf:type owl:DatatypeProperty ;
        rdfs:domain :BodyCharacteristic ;
        rdfs:range xsd:string ;
        rdfs:comment "A property that indicates the age of an individual" ;
        rdfs:label "has age" .


###  http://www.semanticweb.org/user/ontologies/2022/10/untitled-ontology-328#hasAppearence
:hasAppearence rdf:type owl:DatatypeProperty ;
               rdfs:domain :State ;
               rdfs:range xsd:string ;
               rdfs:comment """A property that indiciates the appearence of an instance.
Instance is an entity that could be skin cancer or not""" ;
               rdfs:label "has appearence" .


###  http://www.semanticweb.org/user/ontologies/2022/10/untitled-ontology-328#hasBump
:hasBump rdf:type owl:DatatypeProperty ;
         rdfs:domain :Shape ;
         rdfs:range xsd:boolean ;
         rdfs:comment """A property that idiciates if an instance is a bump or not.
Instance is an entity that could be skin cancer or not""" ;
         rdfs:label "has bump" .


###  http://www.semanticweb.org/user/ontologies/2022/10/untitled-ontology-328#hasChange
:hasChange rdf:type owl:DatatypeProperty ;
           rdfs:domain :Colour ,
                       :Shape ,
                       :Size ;
           rdfs:range xsd:boolean ;
           rdfs:comment "A property that indicates the change in the size, the shape, and the colour of an instance (i.e., skin cancer or potenital skin cancer)" ;
           rdfs:label "has change" .


###  http://www.semanticweb.org/user/ontologies/2022/10/untitled-ontology-328#hasElasticity
:hasElasticity rdf:type owl:DatatypeProperty ;
               rdfs:domain :State ;
               rdfs:range xsd:boolean ;
               rdfs:comment """A property that indiciates if an instance is elastic or not.
Instance is an entity that could be skin cancer or not""" ;
               rdfs:label "has elasticity" .


###  http://www.semanticweb.org/user/ontologies/2022/10/untitled-ontology-328#hasEyeColour
:hasEyeColour rdf:type owl:DatatypeProperty ;
              rdfs:domain :BodyCharacteristic ;
              rdfs:range xsd:string ;
              rdfs:comment "A property that indicates the eye colour of a body" ;
              rdfs:label "has eye colour" .


###  http://www.semanticweb.org/user/ontologies/2022/10/untitled-ontology-328#hasFreckle
:hasFreckle rdf:type owl:DatatypeProperty ;
            rdfs:domain :SkinType ;
            rdfs:range xsd:string ;
            rdfs:comment "A property that indiciates if a skin type has freckles or not" ;
            rdfs:label "has freckle" .


###  http://www.semanticweb.org/user/ontologies/2022/10/untitled-ontology-328#hasGender
:hasGender rdf:type owl:DatatypeProperty ;
           rdfs:domain :BodyCharacteristic ;
           rdfs:range xsd:string ;
           rdfs:comment "A property that indicates the gender of the individual" ;
           rdfs:label "has gender" .


###  http://www.semanticweb.org/user/ontologies/2022/10/untitled-ontology-328#hasHairColour
:hasHairColour rdf:type owl:DatatypeProperty ;
               rdfs:domain :BodyCharacteristic ;
               rdfs:range xsd:string ;
               rdfs:comment "A property that indicates the hair colour of a body" ;
               rdfs:label "has hair colour" .


###  http://www.semanticweb.org/user/ontologies/2022/10/untitled-ontology-328#hasIrregularEdge
:hasIrregularEdge rdf:type owl:DatatypeProperty ;
                  rdfs:domain :Shape ;
                  rdfs:range xsd:boolean ;
                  rdfs:comment """A property that indiciates if an instance has irregular size or not.
Instance is an entity that could be skin cancer or not""" ;
                  rdfs:label "has irregular edge" .


###  http://www.semanticweb.org/user/ontologies/2022/10/untitled-ontology-328#hasItch
:hasItch rdf:type owl:DatatypeProperty ;
         rdfs:domain :State ;
         rdfs:range xsd:boolean ;
         rdfs:comment """A property that indiciates if an instance has itch or not.
Instance is an entity that could be skin cancer or not""" ;
         rdfs:label "has itch" .


###  http://www.semanticweb.org/user/ontologies/2022/10/untitled-ontology-328#hasMelanoma
:hasMelanoma rdf:type owl:DatatypeProperty ;
             rdfs:domain :FamilyHistory ;
             rdfs:range xsd:boolean ;
             rdfs:comment "A property that indicates if an individual had a melanoma in the past" ;
             rdfs:label "had melanoma" .


###  http://www.semanticweb.org/user/ontologies/2022/10/untitled-ontology-328#hasPercussion
:hasPercussion rdf:type owl:DatatypeProperty ;
               rdfs:domain :State ;
               rdfs:range xsd:boolean ;
               rdfs:comment """A property that indiciates if an instance has percussion or not.
Instance is an entity that could be skin cancer or not""" ;
               rdfs:label "has percussion" .


###  http://www.semanticweb.org/user/ontologies/2022/10/untitled-ontology-328#hasVisibleBloodVessel
:hasVisibleBloodVessel rdf:type owl:DatatypeProperty ;
                       rdfs:domain :State ;
                       rdfs:range xsd:string ;
                       rdfs:comment """A property that indiciates if an instance has visible blood vessel or not.
Instance is an entity that could be skin cancer or not""" ;
                       rdfs:label "has visible blood vessels" .


###  http://www.semanticweb.org/user/ontologies/2022/10/untitled-ontology-328#hasWaxyLump
:hasWaxyLump rdf:type owl:DatatypeProperty ;
             rdfs:domain :State ;
             rdfs:range xsd:boolean ;
             rdfs:comment """A property that indiciates if an instance has waxy lump or not.
Instance is an entity that could be skin cancer or not""" ;
             rdfs:label "has waxy lump" .


###  http://www.semanticweb.org/user/ontologies/2022/10/untitled-ontology-328#hasWrinkle
:hasWrinkle rdf:type owl:DatatypeProperty ;
            rdfs:domain :State ;
            rdfs:range xsd:string ;
            rdfs:comment """A property that indiciates if an instance has wrinkles or not.
Instance is an entity that could be skin cancer or not""" ;
            rdfs:label "has wrinkle" .


###  http://www.semanticweb.org/user/ontologies/2022/10/untitled-ontology-328#inRadiation
:inRadiation rdf:type owl:DatatypeProperty ;
             rdfs:domain :FamilyHistory ;
             rdfs:range xsd:boolean ;
             rdfs:comment "A property that indicates that an individual goes through radiation treatment" ;
             rdfs:label "in radiation" .


###  http://www.semanticweb.org/user/ontologies/2022/10/untitled-ontology-328#isAssymetric
:isAssymetric rdf:type owl:DatatypeProperty ;
              rdfs:domain :Size ;
              rdfs:range xsd:boolean ;
              rdfs:comment """A property that indiciates if an instance is assymetric or not.
Instance is an entity that could be skin cancer or not""" ;
              rdfs:label "is assymetric" .


###  http://www.semanticweb.org/user/ontologies/2022/10/untitled-ontology-328#isBleeding
:isBleeding rdf:type owl:DatatypeProperty ;
            rdfs:domain :State ;
            rdfs:range xsd:string ;
            rdfs:comment """A property that indiciates if an instance is bleeding or not.
Instance is an entity that could be skin cancer or not""" ;
            rdfs:label "is bleeding" .


###  http://www.semanticweb.org/user/ontologies/2022/10/untitled-ontology-328#isFlatExfoliatingRash
:isFlatExfoliatingRash rdf:type owl:DatatypeProperty ;
                       rdfs:domain :State ;
                       rdfs:range xsd:boolean ;
                       rdfs:comment """A property that indiciates if an instance is a flat exfoliating rash or not.
Instance is an entity that could be skin cancer or not""" ;
                       rdfs:label "is flat exfoliating rash" .


###  http://www.semanticweb.org/user/ontologies/2022/10/untitled-ontology-328#isHealing
:isHealing rdf:type owl:DatatypeProperty ;
           rdfs:domain :State ;
           rdfs:range xsd:string ;
           rdfs:comment """A property that indiciates if an instance is healing or not.
Instance is an entity that could be skin cancer or not""" ;
           rdfs:label "is healing" .


###  http://www.semanticweb.org/user/ontologies/2022/10/untitled-ontology-328#isPainful
:isPainful rdf:type owl:DatatypeProperty ;
           rdfs:domain :State ;
           rdfs:range xsd:boolean ;
           rdfs:comment """A property that indiciates if an instance is painful or not.
Instance is an entity that could be skin cancer or not""" ;
           rdfs:label "is painful" .


###  http://www.semanticweb.org/user/ontologies/2022/10/untitled-ontology-328#isUlcer
:isUlcer rdf:type owl:DatatypeProperty ;
         rdfs:domain :State ;
         rdfs:range xsd:boolean ;
         rdfs:comment """A property that indiciates if an instance is ulcer or not.
Instance is an entity that could be skin cancer or not""" ;
         rdfs:label "is ulcer" .


###  http://www.semanticweb.org/user/ontologies/2022/10/untitled-ontology-328#isWaxyScar
:isWaxyScar rdf:type owl:DatatypeProperty ;
            rdfs:domain :Shape ;
            rdfs:range xsd:boolean ;
            rdfs:comment """A property that indiciates if an instance is waxy scar or not.
Instance is an entity that could be skin cancer or not""" ;
            rdfs:label "is waxy scar" .


###  http://www.semanticweb.org/user/ontologies/2022/10/untitled-ontology-328#isWound
:isWound rdf:type owl:DatatypeProperty ;
         rdfs:domain :State ;
         rdfs:range xsd:string ;
         rdfs:comment """A property that indiciates if an instance has a wound or not.
Instance is an entity that could be skin cancer or not""" ;
         rdfs:label "is wound" .


###  http://www.semanticweb.org/user/ontologies/2022/10/untitled-ontology-328#isofSize
:isofSize rdf:type owl:DatatypeProperty ;
          rdfs:domain :Size ;
          rdfs:range xsd:string ;
          rdfs:comment """A property that indiciates the size of an instance.
Instance is an entity that could be skin cancer or not""" ;
          rdfs:label "is of size" .


###  http://www.semanticweb.org/user/ontologies/2022/10/untitled-ontology-328#located
:located rdf:type owl:DatatypeProperty ;
         rdfs:domain :BodyPart ;
         rdfs:range xsd:string ;
         rdfs:comment """A property that indiciates where on the body the instance is located.
Instance is an entity that could be skin cancer or not""" ;
         rdfs:label "located" .


###  http://www.semanticweb.org/user/ontologies/2022/10/untitled-ontology-328#stateOfImmune
:stateOfImmune rdf:type owl:DatatypeProperty ;
               rdfs:domain :ImmuneSystem ;
               rdfs:range xsd:string ;
               rdfs:comment "A property that indicates the state of the immune system" ;
               rdfs:label "state of immune" .


###  http://www.semanticweb.org/user/ontologies/2022/10/untitled-ontology-328#typeOfSkin
:typeOfSkin rdf:type owl:DatatypeProperty ;
            rdfs:domain :SkinType ;
            rdfs:range xsd:string ;
            rdfs:comment "A property that indicates the type of skin" ;
            rdfs:label "type of skin" .


#################################################################
#    Classes
#################################################################

###  http://www.semanticweb.org/user/ontologies/2022/10/untitled-ontology-328#BasalCell
:BasalCell rdf:type owl:Class ;
           rdfs:subClassOf :CancerType ;
           rdfs:comment "A class for the basal cell skin cancer type" ;
           rdfs:label "Basal Cell Carcinoma" .


###  http://www.semanticweb.org/user/ontologies/2022/10/untitled-ontology-328#BodyCharacteristic
:BodyCharacteristic rdf:type owl:Class ;
                    rdfs:subClassOf :Danger ;
                    rdfs:comment "A class that indicates the body characteristics that increase the chance to suffer skin cancer" ;
                    rdfs:label "body characteristic" .


###  http://www.semanticweb.org/user/ontologies/2022/10/untitled-ontology-328#BodyPart
:BodyPart rdf:type owl:Class ;
          rdfs:comment "A class that indicates the body parts that a skin cancer may appear" ;
          rdfs:label "Body Part" .


###  http://www.semanticweb.org/user/ontologies/2022/10/untitled-ontology-328#CancerType
:CancerType rdf:type owl:Class ;
            rdfs:comment "A class that contains the types of cancer" ;
            rdfs:label "Cancer Type" .


###  http://www.semanticweb.org/user/ontologies/2022/10/untitled-ontology-328#Colour
:Colour rdf:type owl:Class ;
        rdfs:subClassOf :Symptom ;
        rdfs:comment "A property that indicates the colour of an instance (which may or may not be a skin cancer)" ;
        rdfs:label "Colour" .


###  http://www.semanticweb.org/user/ontologies/2022/10/untitled-ontology-328#Danger
:Danger rdf:type owl:Class ;
        rdfs:comment "A class that contains the risk factors that may provoke a skin cancer" ;
        rdfs:label "danger" .


###  http://www.semanticweb.org/user/ontologies/2022/10/untitled-ontology-328#Exposure
:Exposure rdf:type owl:Class ;
          rdfs:subClassOf :Danger ;
          rdfs:comment "A class that indicates the things that when exposed to  increase the chance to suffer skin cancer" ;
          rdfs:label "exposure" .


###  http://www.semanticweb.org/user/ontologies/2022/10/untitled-ontology-328#FamilyHistory
:FamilyHistory rdf:type owl:Class ;
               rdfs:subClassOf :Danger ;
               rdfs:comment "A class that indicates the family history aspects that increase the danger to suffer skin cancer" ;
               rdfs:label "family history" .


###  http://www.semanticweb.org/user/ontologies/2022/10/untitled-ontology-328#ImmuneSystem
:ImmuneSystem rdf:type owl:Class ;
              rdfs:subClassOf :Danger ;
              rdfs:comment "A class that indicates the state of the immune system which increase the chance to suffer skin cancer" ;
              rdfs:label "immune system" .


###  http://www.semanticweb.org/user/ontologies/2022/10/untitled-ontology-328#Melanoma
:Melanoma rdf:type owl:Class ;
          rdfs:subClassOf :CancerType ;
          rdfs:comment "A class for the melanoma skin cancer type" ;
          rdfs:label "Melanoma" .


###  http://www.semanticweb.org/user/ontologies/2022/10/untitled-ontology-328#Shape
:Shape rdf:type owl:Class ;
       rdfs:subClassOf :Symptom ;
       rdfs:comment "A property that indicates the shape of an instance (which may or may not be a skin cancer)" ;
       rdfs:label "Shape" .


###  http://www.semanticweb.org/user/ontologies/2022/10/untitled-ontology-328#Size
:Size rdf:type owl:Class ;
      rdfs:subClassOf :Symptom ;
      rdfs:comment "A property that indicates the size of an instance (which may or may not be a skin cancer)" ;
      rdfs:label "Size" .


###  http://www.semanticweb.org/user/ontologies/2022/10/untitled-ontology-328#SkinType
:SkinType rdf:type owl:Class ;
          rdfs:subClassOf :Danger ;
          rdfs:comment "A class that indicates the skin types that are more dangerous to suffer skin cancer" ;
          rdfs:label "skin type" .


###  http://www.semanticweb.org/user/ontologies/2022/10/untitled-ontology-328#SquamousCell
:SquamousCell rdf:type owl:Class ;
              rdfs:subClassOf :CancerType ;
              rdfs:comment "A class for the squamous cell skin cancer type" ;
              rdfs:label "Squamous Cell Carcinoma" .


###  http://www.semanticweb.org/user/ontologies/2022/10/untitled-ontology-328#State
:State rdf:type owl:Class ;
       rdfs:subClassOf :Symptom ;
       rdfs:comment "State" ;
       rdfs:label "A property that indicates the state of an instance (which may or may not be a skin cancer)" .


###  http://www.semanticweb.org/user/ontologies/2022/10/untitled-ontology-328#Symptom
:Symptom rdf:type owl:Class ;
         rdfs:comment "A class that contains the classes with the symptoms" ;
         rdfs:label "Syptom" .


###  Generated by the OWL API (version 4.5.9.2019-02-01T07:24:44Z) https://github.com/owlcs/owlapi
